src/Parsers/Grammars/ExpressionNumPlusParen.v
@@ -8,7 +8,7 @@ Section num_plus_paren.
   Local Open Scope string_scope.
   Local Open Scope grammar_scope.
 
-  Definition plus_expr_grammar : grammar string :=
+  Definition plus_expr_grammar : grammar Ascii.ascii :=
     [[[ ("expr" ::== << $< "pexpr" >$
                       | $< "pexpr" $ #"+" $ "expr" >$ >>);;
         ("pexpr" ::== << $< "number" >$
@@ -27,9 +27,9 @@ Section tests.
                    | [ |- parse_of_production _ ?s (Terminal _ :: _) ]
                      => apply ParseProductionCons with (n := 1)
                    | [ |- parse_of_production _ ?s (_ :: nil) ]
-                     => apply ParseProductionCons with (n := length s)
+                     => apply ParseProductionCons with (n := String.length s)
                    | [ |- parse_of_production _ ?s (_ :: Terminal _ :: nil) ]
-                     => apply ParseProductionCons with (n := length s - 1)
+                     => apply ParseProductionCons with (n := String.length s - 1)
                     end)
                  | apply ParseProductionNil
                  | refine (ParseTerminal _ _ _)
