src/Parsers/ParserInterface.v
@@ -8,11 +8,11 @@ Local Open Scope list_scope.
 Reserved Infix "~=" (at level 70).
 
 Section interface.
-  Context {string} `{StringLike string} (G : grammar string).
+  Context {Char} (G : grammar Char).
 
   (** A production is reachable if it is the tail of a production
       associated to a valid nonterminal. *)
-  Definition production_is_reachable (p : production string) : Prop
+  Definition production_is_reachable (p : production Char) : Prop
     := exists nt prefix,
          List.In nt (Valid_nonterminals G)
          /\ List.In
@@ -22,7 +22,7 @@ Section interface.
   (** A list of splits is complete if, for every reachable production,
       it contains every index of the string that yields a parse tree
       for that production by splitting at that index. *)
-  Definition split_list_is_complete (str : String) (it : item string) (its : production string)
+  Definition split_list_is_complete `{HSL : StringLike Char} (str : String) (it : item Char) (its : production Char)
              (splits : list nat)
   : Prop
     := forall n,
@@ -34,49 +34,32 @@ Section interface.
 
   Record Splitter :=
     {
-      split_rep : Type;
-      (** metadata associated with the string, to help split it *)
-      split_take : nat -> split_rep -> split_rep;
-      (** take the metadata associated with the first [n] characters *)
-      split_drop : nat -> split_rep -> split_rep;
-      (** take the metadata associated with all but the first [n] characters *)
-      splits_for : split_rep -> item string -> production string -> list nat;
+      string_type :> StringLike Char;
+      splits_for : String -> item Char -> production Char -> list nat;
       (** give a list of indices for splitting a given string *)
 
-      split_invariant : String -> split_rep -> Prop where "s ~= st" := (split_invariant s st);
-      (** invariant relating a [String] to a representation *)
-
-
-      take_respectful : forall str st n,
-                          str ~= st
-                          -> fst (SplitAt n str) ~= split_take n st;
-      (** [split_take] must respect the invariant *)
-      drop_respectful : forall str st n,
-                          str ~= st
-                          -> snd (SplitAt n str) ~= split_drop n st;
-      (** [split_drop] must respect the invariant *)
-      splits_for_complete : forall str st it its,
-                              str ~= st
-                              -> split_list_is_complete str it its (splits_for st it its)
+      string_type_properties :> StringLikeProperties Char;
+      splits_for_complete : forall str it its,
+                              split_list_is_complete str it its (splits_for str it its)
       (** [splits_for] must contain all valid indices for splitting *)
     }.
 
+  Global Existing Instance string_type.
+  Global Existing Instance string_type_properties.
+Set Printing All.
   Record Parser (splitter : Splitter) :=
     {
-      has_parse : String -> split_rep splitter -> bool;
+      has_parse : @String Char splitter -> bool;
       (** does this string parse as the start symbol of the grammar? *)
 
-      has_parse_sound : forall str st,
-                          split_invariant splitter str st
-                          -> has_parse str st = true
-                          -> parse_of_item String G str (NonTerminal _ (Start_symbol G));
+      has_parse_sound : forall str,
+                          has_parse str = true
+                          -> parse_of_item G str (NonTerminal (Start_symbol G));
 
-      has_parse_complete : forall str (p : parse_of_item String G str (NonTerminal _ (Start_symbol G))),
+      has_parse_complete : forall str (p : parse_of_item G str (NonTerminal (Start_symbol G))),
                              Forall_parse_of_item
                                (fun _ nt => List.In nt (Valid_nonterminals G))
                                p
-                             -> forall st,
-                                  split_invariant splitter str st
-                                  -> has_parse str st = true
+                             -> has_parse str = true
     }.
 End interface.
