src/Parsers/StringLike.v
@@ -2,10 +2,10 @@
 (** ** Definitions *)
 Require ADTSynthesis.Parsers.StringLike.Core.
 (** ** Various string-like types *)
-Require ADTSynthesis.Parsers.StringLike.Examples.
+Require ADTSynthesis.Parsers.StringLike.String.
 (** ** Various theorems about string-like types *)
 Require ADTSynthesis.Parsers.StringLike.Properties.
 
 Export Parsers.StringLike.Core.
-Export Parsers.StringLike.Examples.
+Export Parsers.StringLike.String.
 Export Parsers.StringLike.Properties.
